Prove all theorems with only out_ffi related cheats remaining

pancake/proofs/ntime_to_panProofScript.sml
@@ -278,7 +278,7 @@ Proof
   cases_on ‘i’ >>
   gs []
   >- (
-    (* delay input *)
+    (* input step *)
     gs [steps_def] >>
     gs [assumptions_def, event_inv_def, ffi_rels_def, ffi_rel_def] >>
     rveq >> gs [] >>
@@ -341,478 +341,56 @@ Proof
     impl_tac
     >- gs [action_rel_def, ffiTimeTheory.next_ffi_def] >>
     gs []) >>
-
-
-QED
-
-(*
-Definition local_action_def:
-  (local_action (Input i) t =
-     (FLOOKUP t.locals «isInput» = SOME (ValWord 0w))) ∧
-  (local_action (Output os) t =
-    (FLOOKUP t.locals «event»   = SOME (ValWord 0w) ∧
-     FLOOKUP t.locals «isInput» = SOME (ValWord 1w) ∧
-     FLOOKUP t.locals «waitSet» = SOME (ValWord 0w)))
-End
-
-Definition local_state_def:
-  (local_state (LDelay _) t =
-   (FLOOKUP t.locals «isInput» = SOME (ValWord 1w) ∧
-    FLOOKUP t.locals «event» = SOME (ValWord 0w))) ∧
-  (local_state (LAction act) t = local_action act t)
-End
-
-Definition locals_def:
-  (locals [] t = T) ∧
-  (locals (lbl::lbls) t = local_state lbl t)
-End
-*)
-
-
-(*
-Definition evaluations_def:
-  (evaluations prog [] t ⇔ T) ∧
-  (evaluations prog (lbl::lbls) t ⇔
-   ∃ck nt.
-     evaluate (always (nClks prog), t with clock := t.clock + ck) =
-     evaluate (always (nClks prog), nt) ∧
-     evaluations prog lbls nt)
-End
-
-
-Definition evaluation_invs_def:
-  (evaluation_inv prog [] s (t:('a,time_input) panSem$state) ⇔ T) ∧
-  (evaluation_inv prog (lbl::lbls) s t ⇔
-   ∃m n st nt.
-     step prog lbl m n s st ∧
-     evaluate (always (nClks prog), t) =
-     evaluate (always (nClks prog), nt) ⇒
-     state_rel (clksOf prog) st nt ∧
-     nt.code = t.code ∧
-     next_ffi_state lbl t.ffi.ffi_state nt.ffi.ffi_state ∧
-     nt.ffi.oracle = t.ffi.oracle ∧
-     nlocals lbl nt.locals (t.ffi.ffi_state) st.waitTime (dimword (:α)) ∧
-     task_ret_defined nt.locals (nClks prog) ∧
-     evaluation_inv prog lbls st nt)
-End
-*)
-
-
-(*
-Definition evaluate_rel_def:
-  (evaluate_rel prog lbl t nt ⇔
-   case lbl of
-   | LDelay d =>
-       evaluate (task_controller (nClks prog), t) =
-       evaluate (task_controller (nClks prog), nt)
-   | LAction _ =>
-       evaluate (task_controller (nClks prog), t) =
-       (NONE, nt))
-End
-
-
-Definition evaluations_def:
-  (evaluations prog [] t ⇔ T) ∧
-  (evaluations prog (lbl::lbls) t ⇔
-   ∃nt.
-     evaluate_rel prog lbl t nt ∧
-     evaluations prog lbls nt) ∧
-  (evaluations prog _ t ⇔ T)
-End
-*)
-
-(*
-(*
-Definition event_state_def:
-  event_state t ⇔
-    FLOOKUP t.locals «isInput» = SOME (ValWord 1w) ∧
-    FLOOKUP t.locals «event»   =  SOME (ValWord 0w)
-End
-
-Definition evaluations_def:
-  (evaluations prog t [] [] ⇔ T) ∧
-  (evaluations prog t (lbl::lbls) (nt::nts) ⇔
-     evaluate_rel prog lbl t nt ∧
-     evaluations prog nt lbls nts) ∧
-  (evaluations prog t _ _ ⇔ T)
-End
-
-Definition state_rels_def:
-  (state_rels prog [] s t ⇔ T) ∧
-  (state_rels prog (lbl::lbls) s t ⇔
-   ∀m n st nt.
-     step prog lbl m n s st ∧
-     evaluate_rel prog lbl t nt ⇒
-     state_rel (clksOf prog) st nt ∧
-     state_rels prog lbls st nt)
-End
-
-Definition always_code_installed_def:
-  (always_code_installed prog [] t ⇔ T) ∧
-  (always_code_installed prog (lbl::lbls) t ⇔
-   ∀nt.
-     evaluate_rel prog lbl t nt ⇒
-     code_installed nt.code prog ∧
-     always_code_installed prog lbls nt)
-End
-*)
-
-
-Theorem foo:
-  ∀prog s s' labels (t:('a,time_input) panSem$state).
-    stepTrace prog
-              (dimword (:α) - 1)
-              (FST (t.ffi.ffi_state 0)) s s' labels ∧
-    state_rel (clksOf prog) s t ∧
-    code_installed t.code prog ∧
-    well_formed_code prog t.code ∧
-    out_ffi prog t ∧
-    ffi_rels prog labels s t ∧
-    labProps$good_dimindex (:'a) ∧
-    local_state (HD labels) t ∧
-    (* we shoud be able to prove that this stays as an invariant
-       after each invocation of the task *)
-    (* should we assume that labels are non-empty *)
-    task_ret_defined t.locals (nClks prog) ⇒
-    ?ck t'.
-      evaluate (always (nClks prog), t with clock := t.clock + ck) =
-      evaluate (always (nClks prog), t') ∧
-      state_rel (clksOf prog) s' t' ∧
-      code_installed t'.code prog
-Proof
-QED
-
-
-
-
-
-(*
-Definition next_wakeup_def:
-  (next_wakeup (LDelay _) (t:('a,time_input) panSem$state) (t':('a,time_input) panSem$state) =
-   (FLOOKUP t'.locals «wakeUpAt» = FLOOKUP t.locals «wakeUpAt»)) ∧
-  (next_wakeup (LAction _) t t' =
-   (t'.ffi.ffi_state = t.ffi.ffi_state ∧
-    (∃wt.
-       FLOOKUP t'.locals «wakeUpAt» =
-       SOME (ValWord (n2w (FST (t.ffi.ffi_state 0) + wt))) ∧
-       FST (t.ffi.ffi_state 0) + wt < dimword (:α))))
-End
-*)
-
-
-(*
-Theorem step_thm:
-  !prog label s s' (t:('a,time_input) panSem$state) ck_extra.
-    step prog label s s' ∧
-    state_rel (clksOf prog) s t ∧
-    code_installed t.code prog ∧
-    labProps$good_dimindex (:'a) ⇒
-    case label of
-    | LDelay d =>
-        ∀cycles.
-          delay_rep (dimword (:α)) d t.ffi.ffi_state cycles ∧
-          wakeup_rel t.locals (dimword (:α)) s.waitTime t.ffi.ffi_state cycles ∧
-          mem_read_ffi_results (:α) t.ffi.ffi_state cycles ∧
-          FLOOKUP t.locals «isInput» = SOME (ValWord 1w) ⇒
-          ?ck t'.
-            evaluate (task_controller (nClks prog), t with clock := t.clock + ck) =
-            evaluate (task_controller (nClks prog), t' with clock := t'.clock + ck_extra) ∧
-            code_installed t'.code prog ∧
-            state_rel (clksOf prog) s' t' ∧
-            t'.ffi.ffi_state = nexts_ffi cycles t.ffi.ffi_state ∧
-            t'.ffi.oracle = t.ffi.oracle ∧
-            FLOOKUP t'.locals «wakeUpAt» = FLOOKUP t.locals «wakeUpAt» ∧
-            FLOOKUP t'.locals «isInput» = SOME (ValWord 1w) ∧
-            FLOOKUP t'.locals «sysTime»  =
-            SOME (ValWord (n2w (FST (t.ffi.ffi_state cycles))))
-    | LAction (Input i) =>
-        well_formed_terms prog s t ∧
-        input_rel t.locals (dimword (:α)) i t.ffi.ffi_state ∧
-        FLOOKUP t.locals «isInput» = SOME (ValWord 0w) ∧
-        task_ret_defined t.locals (nClks prog) ⇒
-        ?ck t'.
-          evaluate (task_controller (nClks prog), t with clock := t.clock + ck) =
-          (NONE, t') ∧
-          code_installed t'.code prog ∧
-          state_rel (clksOf prog) s' t' ∧
-          t'.ffi.ffi_state = t.ffi.ffi_state ∧
-          t'.ffi.oracle = t.ffi.oracle ∧
-          FLOOKUP t'.locals «sysTime» = FLOOKUP t.locals «sysTime» ∧
-          FLOOKUP t'.locals «event»   = SOME (ValWord 0w) ∧
-          FLOOKUP t'.locals «isInput» = SOME (ValWord 1w) ∧
-          task_ret_defined t'.locals (nClks prog) ∧
-          (∃wt.
-             FLOOKUP t'.locals «wakeUpAt» =
-             SOME (ValWord (n2w (FST (t.ffi.ffi_state 0) + wt))) ∧
-             FST (t.ffi.ffi_state 0) + wt < dimword (:α))
-    | LAction (Output os) =>
-        well_formed_terms prog s t ∧
-        output_rel t.locals (dimword (:α)) s.waitTime t.ffi.ffi_state ∧
-        FLOOKUP t.locals «event»   = SOME (ValWord 0w) ∧
-        FLOOKUP t.locals «isInput» = SOME (ValWord 1w) ∧
-        FLOOKUP t.locals «waitSet» = SOME (ValWord 0w) ∧
-        task_ret_defined t.locals (nClks prog) ∧
-        (∃tt. s.waitTime = SOME tt) ⇒
-        ?ck t'.
-          evaluate (task_controller (nClks prog), t with clock := t.clock + ck) =
-          (NONE, t') ∧
-          code_installed t'.code prog ∧
-          state_rel (clksOf prog) s' t' ∧
-          t'.ffi.ffi_state = t.ffi.ffi_state ∧
-          t'.ffi.oracle = t.ffi.oracle ∧
-          FLOOKUP t'.locals «sysTime» = FLOOKUP t.locals «sysTime» ∧
-          FLOOKUP t'.locals «event»   = SOME (ValWord 0w) ∧
-          FLOOKUP t'.locals «isInput» = SOME (ValWord 1w) ∧
-          task_ret_defined t'.locals (nClks prog) ∧
-          (∃wt.
-             FLOOKUP t'.locals «wakeUpAt» =
-             SOME (ValWord (n2w (FST (t.ffi.ffi_state 0) + wt))) ∧
-             FST (t.ffi.ffi_state 0) + wt < dimword (:α))
-Proof
-  rw [] >>
-  cases_on ‘label’ >>
-  fs []
-  >- (
-    rw [] >>
-    drule_all step_delay >>
-    disch_then (qspec_then ‘ck_extra’ mp_tac) >>
-    fs []) >>
-  cases_on ‘i’
-  >- (
-    fs [] >>
-    rw [] >>
-    drule_all step_input >>
-    disch_then (qspec_then ‘ck_extra’ mp_tac) >>
-    fs []) >>
-  fs [] >>
-  rw [] >>
+  (* output step *)
+  gs [steps_def] >>
+  gs [assumptions_def, event_inv_def, ffi_rels_def, ffi_rel_def] >>
+  rveq >> gs [] >>
   drule step_output >>
-  disch_then (qspec_then ‘t’ mp_tac) >>
-  fs []
-QED
-*)
-
-
-
-
-(*
-Definition well_formness_def:
-  (well_formness (LDelay _) prog s (t:('a,time_input) panSem$state) = T) ∧
-  (well_formness (LAction _) prog s t =
-   (well_formed_terms prog s t ∧ task_ret_defined t.locals (nClks prog)))
-End
-*)
-
-
-
-Theorem step_delay_weaker:
-  !prog d s s' (t:('a,time_input) panSem$state).
-    step prog (LDelay d) s s' ∧
-    state_rel (clksOf prog) s t ∧
-    code_installed t.code prog ∧
-    ffi_rel (LDelay d) s t ∧
-    local_state (LDelay d) t ∧
-    code_installed t.code prog ∧
-    labProps$good_dimindex (:'a) ∧
-    (* extra assumptions *)
-    task_ret_defined t.locals (nClks prog) ∧
-    well_formed_terms prog s t ⇒
-    ?ck t'.
-      evaluate (task_controller (nClks prog), t with clock := t.clock + ck) =
-      evaluate (task_controller (nClks prog), t') ∧
-      state_rel (clksOf prog) s' t' ∧
-      code_installed t'.code prog ∧
-      next_wakeup (LDelay d) t t' ∧
-      event_state t' ∧
-      task_ret_defined t'.locals (nClks prog) ∧
-      well_formed_terms prog s' t'
-Proof
-  rw [] >>
-  fs [ffi_rel_def] >>
-  drule step_delay >>
-  disch_then (qspecl_then [‘cycles’, ‘t’, ‘0’] mp_tac) >>
-  impl_tac
-  >- gs [local_state_def] >>
-  strip_tac >>
-  qexists_tac ‘ck’ >>
-  qexists_tac ‘t'’ >>
   gs [] >>
-  ‘t' with clock := t'.clock = t'’ by
-    fs [state_component_equality] >>
-  gs [next_wakeup_def, event_state_def, local_state_def] >>
-  gs [task_ret_defined_def] >>
-  fs [step_cases]
+  disch_then (qspec_then ‘t’ mp_tac) >>
+  impl_tac
   >- (
-    gs [well_formed_terms_def, mkState_def] >>
-    gen_tac >>
-    strip_tac >>
-    first_x_assum drule >>
-    strip_tac >>
-    gs [resetOutput_def] >>
-    conj_tac
-    >- (
-      gs [conds_eval_lt_dimword_def] >>
-      gs [EVERY_MEM] >>
-      rw [] >>
-      first_x_assum drule_all >>
-      gs []  >>
-      TOP_CASE_TAC >> gs [] >>
-      strip_tac >>
-      cheat) >>
-    (* this is complicated *)
-    conj_tac
-    >- cheat >>
+    gs [compactDSLSemTheory.step_cases] >>
+    gs [well_formed_code_def] >>
+    gs [action_rel_def] >>
+    (* out_ffi cheat *)
     cheat) >>
-  cheat
-QED
-
-Theorem step_input_weaker:
-  !prog i s s' (t:('a,time_input) panSem$state).
-    step prog (LAction (Input i)) s s' ∧
-    state_rel (clksOf prog) s t ∧
-    code_installed t.code prog ∧
-    ffi_rel (LAction (Input i)) s t ∧
-    local_state (LAction (Input i)) t ∧
-    code_installed t.code prog ∧
-    labProps$good_dimindex (:'a) ∧
-    (* extra assumptions *)
-    task_ret_defined t.locals (nClks prog) ∧
-    well_formed_terms prog s t ⇒
-    ?ck t'.
-      evaluate (task_controller (nClks prog), t with clock := t.clock + ck) =
-      (NONE, t') ∧
-      state_rel (clksOf prog) s' t' ∧
-      code_installed t'.code prog ∧
-      next_wakeup (LAction (Input i)) t t' ∧
-      event_state t' ∧
-      task_ret_defined t'.locals (nClks prog) ∧
-      well_formed_terms prog s' t'
-Proof
-  rw [] >>
-  fs [ffi_rel_def] >>
-  drule step_input >>
-  disch_then (qspec_then ‘t’ mp_tac) >>
-  impl_tac
-  >- gs [action_rel_def, local_state_def, local_action_def] >>
   strip_tac >>
-  qexists_tac ‘ck’ >>
-  qexists_tac ‘t'’ >>
+  gs [evaluations_def, event_inv_def] >>
+  qexists_tac ‘ck+1’ >>
+  gs [always_def] >>
+  rewrite_tac [Once panSemTheory.evaluate_def] >>
+  gs [panSemTheory.eval_def] >>
+  gs [panSemTheory.dec_clock_def] >>
+  qexists_tac ‘t''’ >>
+  fs [] >>
+  MAP_EVERY qexists_tac [‘dimword (:α) − 1’,‘FST (t.ffi.ffi_state 0)’,‘h'’] >>
   gs [] >>
-  conj_tac
+  conj_asm1_tac
+  >- gs [next_ffi_state_def] >>
+  gs [nlocals_def] >>
+  conj_asm1_tac
   >- (
-    gs [next_wakeup_def] >>
-    qexists_tac ‘wt’ >> gs []) >>
-  conj_tac
-  >- gs [event_state_def] >>
-  gs [well_formed_terms_def]  >>
-  gen_tac >>
-  strip_tac >>
-  (* need more assumptions *)
-  cheat
-QED
-
-
-Theorem step_output_weaker:
-  !prog os s s' (t:('a,time_input) panSem$state).
-    step prog (LAction (Output os)) s s' ∧
-    state_rel (clksOf prog) s t ∧
-    code_installed t.code prog ∧
-    ffi_rel (LAction (Output os)) s t ∧
-    local_state (LAction (Output os)) t ∧
-    code_installed t.code prog ∧
-    labProps$good_dimindex (:'a) ∧
-    (* should be rephrased *)
-    (∃tt. s.waitTime = SOME tt) ∧
-    (* extra assumptions *)
-    task_ret_defined t.locals (nClks prog) ∧
-    well_formed_terms prog s t ⇒
-    ?ck t'.
-      evaluate (task_controller (nClks prog), t with clock := t.clock + ck) =
-      (NONE, t') ∧
-      state_rel (clksOf prog) s' t' ∧
-      code_installed t'.code prog ∧
-      next_wakeup (LAction (Output os)) t t' ∧
-      event_state t' ∧
-      task_ret_defined t'.locals (nClks prog) ∧
-      well_formed_terms prog s' t'
-Proof
-  rw [] >>
-  fs [ffi_rel_def] >>
-  drule step_output >>
-  disch_then (qspec_then ‘t’ mp_tac) >>
-  impl_tac
-  >- gs [action_rel_def, local_state_def, local_action_def] >>
-  strip_tac >>
-  qexists_tac ‘ck’ >>
-  qexists_tac ‘t'’ >>
+  cases_on ‘h'.waitTime’ >>
+  gs [wait_time_locals_def]
+  >- (
+    qexists_tac ‘0’ >>
+    qexists_tac ‘FST (t.ffi.ffi_state 0)’ >>
+    gs [compactDSLSemTheory.step_cases]) >>
+  qexists_tac ‘x’ >>
+  qexists_tac ‘FST (t.ffi.ffi_state 0)’ >>
+  gs []) >>
+  last_x_assum match_mp_tac >>
   gs [] >>
+  qexists_tac ‘t'’ >>
+  gs [ffiTimeTheory.next_ffi_def] >>
   conj_tac
-  >- (
-    gs [next_wakeup_def] >>
-    qexists_tac ‘wt’ >> gs []) >>
-  conj_tac
-  >- gs [event_state_def] >>
-  gs [well_formed_terms_def]  >>
-  gen_tac >>
-  strip_tac >>
-  (* need more assumptions *)
-  cheat
+  (* out_ffi cheat *)
+  >- cheat >>
+  first_x_assum drule >>
+  disch_then (qspec_then ‘t''’ mp_tac) >>
+  impl_tac
+  >- gs [action_rel_def, ffiTimeTheory.next_ffi_def] >>
+  gs []
 QED
-
-
-(*
-Definition next_wakeup_def:
-  (next_wakeup (LDelay _) (t:('a,time_input) panSem$state) (t':('a,time_input) panSem$state) =
-   (FLOOKUP t'.locals «waitSet» = SOME (ValWord 0w) ∧
-    FLOOKUP t'.locals «wakeUpAt» = FLOOKUP t.locals «wakeUpAt»)) ∧
-  (next_wakeup (LAction _) t t' =
-   (t'.ffi.ffi_state = t.ffi.ffi_state ∧
-    FLOOKUP t'.locals «waitSet» = SOME (ValWord 0w) ∧
-    (∃wt.
-       FLOOKUP t'.locals «wakeUpAt» =
-       SOME (ValWord (n2w (FST (t.ffi.ffi_state 0) + wt))) ∧
-       FST (t.ffi.ffi_state 0) + wt < dimword (:α))))
-End
-
-
-Definition eventual_wakeup_def:
-  eventual_wakeup prog <=>
-  let tms = FLAT (MAP SND prog) in
-    EVERY (λtm.
-            ∃h t. termWaitTimes tm = h::t)
-          tms
-End
-*)
-
-
-
-(* start from here *)
-(*
- While (Const 1w)
-             (task_controller clksLength)
-*)
-(* should we talk about number of states, more like a trace
-   sts: list of reachable timeSem state
-   ts: list of states,
-
-   what exactly do we need∃ *)
-Theorem foo:
-  ∀prog s s' labels (t:('a,time_input) panSem$state).
-    stepTrace prog s s' labels ∧
-    state_rel (clksOf prog) s t ∧
-    code_installed t.code prog ∧
-    ffi_rels labels prog s t ∧
-    labProps$good_dimindex (:'a) ∧
-    (* everything is declared *)
-    (* add more updates later *) ⇒
-    ?ck t'.
-      evaluate (always (nClks prog), t with clock := t.clock + ck) =
-      evaluate (always (nClks prog), t') ∧
-      state_rel (clksOf prog) s' t' ∧
-      code_installed t'.code prog
-Proof
-QED
-
-*)
-
 val _ = export_theory();
